nontermination stuff from nontermination2 branchy

bedrock2/src/bedrock2/Semantics.v
@@ -143,72 +143,119 @@ Module exec. Section WithParams.
   Section WithEnv.
   Context (e: env).
 
-  Implicit Types post : trace -> mem -> locals -> Prop. (* COQBUG: unification finds Type instead of Prop and fails to downgrade *)
-  Inductive exec: cmd -> trace -> mem -> locals ->
-                  (trace -> mem -> locals -> Prop) -> Prop :=
+  Inductive mids_and_post :=
+  | postcond (post: forall (q: bool) (t : trace) (m : mem) (l : locals), Prop)
+  | and_then
+      (first_this_happens : forall (q: bool) (t: trace) (m : mem) (l : locals), Prop)
+      (and_then_later_this_happens : forall (q : bool) (t: trace) (m : mem) (l : locals), forall (idx: nat), mids_and_post).
+
+  Record state := { q: bool; t: trace; m: mem; l: locals }.
+  Definition appl_to_state {T: Type} (f : _ -> _ -> _ -> _ -> T) st := f st.(q) st.(t) st.(m) st.(l).
+  Definition state_satisfies (st: state) (post: _ -> _ -> _ -> _ -> Prop) :=
+    appl_to_state post st.
+  
+  (*this fixpoint answers the question: when does an exectution
+    (infinite sequence of states) satisfy a postcondition?*)
+  (*this isn't actually used anywhere for now.  it is mainly documentation.*)
+  Fixpoint interp_mids_and_post (P : mids_and_post) : (nat -> state) -> Prop :=
+    fun f =>
+      match P with
+      | postcond post => exists n, state_satisfies (f n) post
+      | and_then noww later => exists n, state_satisfies (f n) noww /\
+                                     let later := appl_to_state later (f n) in
+                                     forall m,
+                                       interp_mids_and_post (later m) f
+      end.
+
+  (*suffix_good says, given a state after prefix stuff finishes executing, whether the given postcondition holds*)
+  (*idk how to explain what this fixpoint does without reference to seq.*)
+  (*preconditions:
+    - s1 satisfies `prefix`
+    - forall q t m l post', if suffix_good q t m l post' is inhabited, then
+      executing state s2 starting from state (q,t,m,l) will satisfy post'
+   postcondition:
+    - if return value (a Prop) is inhabited, then (seq s1 s2) satisfies `whole`
+   *)
+  Fixpoint sat (prefix: mids_and_post) (suffix_good: bool -> trace -> mem -> locals -> mids_and_post -> Prop) (whole : mids_and_post) : Prop :=
+    match prefix, whole with
+    | postcond post, _ => (forall q t m l, post q t m l -> suffix_good q t m l whole)
+    | and_then mid1 prefix', and_then mid2 whole' =>
+        (forall q t m l, mid1 q t m l -> mid2 q t m l) /\
+          (forall q t m l n, sat (prefix' q t m l n) suffix_good (whole' q t m l n))
+    | _, _ => False
+    end.
+  
+  Inductive exec: cmd -> bool -> trace -> mem -> locals -> mids_and_post -> Prop :=
   | skip: forall t m l post,
-      post t m l ->
-      exec cmd.skip t m l post
+      post true t m l ->
+      exec cmd.skip true t m l (postcond post)
   | set: forall x e t m l post v,
       eval_expr m l e = Some v ->
-      post t m (map.put l x v) ->
-      exec (cmd.set x e) t m l post
+      post true t m (map.put l x v) ->
+      exec (cmd.set x e) true t m l (postcond post)
   | unset: forall x t m l post,
-      post t m (map.remove l x) ->
-      exec (cmd.unset x) t m l post
+      post true t m (map.remove l x) ->
+      exec (cmd.unset x) true t m l (postcond post)
   | store: forall sz ea ev t m l post a v m',
       eval_expr m l ea = Some a ->
       eval_expr m l ev = Some v ->
       store sz m a v = Some m' ->
-      post t m' l ->
-      exec (cmd.store sz ea ev) t m l post
+      post true t m' l ->
+      exec (cmd.store sz ea ev) true t m l (postcond post)
+  | seq: forall c1 c2 t m l prefix post mid,
+      exec c1 true t m l prefix ->
+      (forall q' t' m' l' post', mid q' t' m' l' post' -> exec c2 q' t' m' l' post') ->
+      sat prefix mid post ->
+      exec (cmd.seq c1 c2) true t m l post
+  | while_true: forall e c t m l v prefix post mid,
+      eval_expr m l e = Some v ->
+      word.unsigned v <> 0 ->
+      exec c true t m l prefix ->
+      (forall q' t' m' l' post', mid q' t' m' l' post' -> exec (cmd.while e c) q' t' m' l' post') ->
+      sat prefix mid post ->
+      exec (cmd.while e c) true t m l post
+  | while_false: forall e c t m l post v,
+      eval_expr m l e = Some v ->
+      word.unsigned v = 0 ->
+      post true t m l ->
+      exec (cmd.while e c) true t m l (postcond post)
   | stackalloc: forall x n body t mSmall l post,
       Z.modulo n (bytes_per_word width) = 0 ->
       (forall a mStack mCombined,
         anybytes a n mStack ->
         map.split mCombined mSmall mStack ->
-        exec body t mCombined (map.put l x a)
-          (fun t' mCombined' l' =>
-            exists mSmall' mStack',
-              anybytes a n mStack' /\
-              map.split mCombined' mSmall' mStack' /\
-              post t' mSmall' l')) ->
-      exec (cmd.stackalloc x n body) t mSmall l post
-  | if_true: forall t m l e c1 c2 post v,
-      eval_expr m l e = Some v ->
-      word.unsigned v <> 0 ->
-      exec c1 t m l post ->
-      exec (cmd.cond e c1 c2) t m l post
-  | if_false: forall e c1 c2 t m l post v,
-      eval_expr m l e = Some v ->
-      word.unsigned v = 0 ->
-      exec c2 t m l post ->
-      exec (cmd.cond e c1 c2) t m l post
-  | seq: forall c1 c2 t m l post mid,
-      exec c1 t m l mid ->
-      (forall t' m' l', mid t' m' l' -> exec c2 t' m' l' post) ->
-      exec (cmd.seq c1 c2) t m l post
-  | while_false: forall e c t m l post v,
-      eval_expr m l e = Some v ->
-      word.unsigned v = 0 ->
-      post t m l ->
-      exec (cmd.while e c) t m l post
-  | while_true: forall e c t m l post v mid,
-      eval_expr m l e = Some v ->
-      word.unsigned v <> 0 ->
-      exec c t m l mid ->
-      (forall t' m' l', mid t' m' l' -> exec (cmd.while e c) t' m' l' post) ->
-      exec (cmd.while e c) t m l post
-  | call: forall binds fname arges t m l post params rets fbody args lf mid,
-      map.get e fname = Some (params, rets, fbody) ->
-      eval_call_args m l arges = Some args ->
-      map.of_list_zip params args = Some lf ->
-      exec fbody t m lf mid ->
-      (forall t' m' st1, mid t' m' st1 ->
-          exists retvs, map.getmany_of_list st1 rets = Some retvs /\
-          exists l', map.putmany_of_list_zip binds retvs l = Some l' /\
-          post t' m' l') ->
-      exec (cmd.call binds fname arges) t m l post
+        exists prefix,
+        exec body true t mCombined (map.put l x a) prefix /\
+        sat
+          prefix
+          (fun q' t' mCombined' l' suffix =>
+             exists post', suffix = postcond post' /\
+                        exists mSmall' mStack',
+                          anybytes a n mStack' /\
+                            map.split mCombined' mSmall' mStack' /\
+                            post' q' t' mSmall' l')
+          post) ->
+      exec (cmd.stackalloc x n body) true t mSmall l post
+  (* | if_true: forall t m l e c1 c2 post v, *)
+  (*     eval_expr m l e = Some v -> *)
+  (*     word.unsigned v <> 0 -> *)
+  (*     exec c1 true t m l post -> *)
+  (*     exec (cmd.cond e c1 c2) true t m l post *)
+  (* | if_false: forall e c1 c2 t m l post v, *)
+  (*     eval_expr m l e = Some v -> *)
+  (*     word.unsigned v = 0 -> *)
+  (*     exec c2 true t m l post -> *)
+  (*     exec (cmd.cond e c1 c2) true t m l post *)
+  (* | call: forall binds fname arges t m l post params rets fbody args lf mid, *)
+  (*     map.get e fname = Some (params, rets, fbody) -> *)
+  (*     eval_call_args m l arges = Some args -> *)
+  (*     map.of_list_zip params args = Some lf -> *)
+  (*     exec fbody true t m lf mid -> *)
+  (*     (forall q' t' m' st1, mid q' t' m' st1 -> *)
+  (*         exists retvs, map.getmany_of_list st1 rets = Some retvs /\ *)
+  (*         exists l', map.putmany_of_list_zip binds retvs l = Some l' /\ *)
+  (*         post q' t' m' l') -> *)
+  (*     exec (cmd.call binds fname arges) true t m l post *)
   | interact: forall binds action arges args t m l post mKeep mGive mid,
       map.split m mKeep mGive ->
       eval_call_args m l arges = Some args ->
@@ -216,170 +263,397 @@ Module exec. Section WithParams.
       (forall mReceive resvals, mid mReceive resvals ->
           exists l', map.putmany_of_list_zip binds resvals l = Some l' /\
           forall m', map.split m' mKeep mReceive ->
-          post (cons ((mGive, action, args), (mReceive, resvals)) t) m' l') ->
-      exec (cmd.interact binds action arges) t m l post.
+          post true (cons ((mGive, action, args), (mReceive, resvals)) t) m' l') ->
+      exec (cmd.interact binds action arges) true t m l (postcond post)
+  | quit: forall c q t m l post,
+      post false t m l ->
+      exec c q t m l (postcond post)
+  | mid: forall c q t m l mid post,
+      mid q t m l ->
+      (*the quantifier here slipped past the nondeterminism! this is the whole point*)
+      (forall n, exec c q t m l (post q t m l n)) ->
+      exec c q t m l (and_then mid post).
 
-  Context {word_ok: word.ok word} {mem_ok: map.ok mem} {ext_spec_ok: ext_spec.ok ext_spec}.
+  Lemma seq_cps_sorta c1 c2 t m l prefix post :
+    exec c1 true t m l prefix ->
+    sat prefix (exec c2) post ->
+    exec (cmd.seq c1 c2) true t m l post.
+  Proof.
+    intros. eapply seq with (mid := exec c2). 1: eassumption. 1: auto. 1: assumption.
+  Qed.
 
+  Lemma seq_cps_for_real c1 c2 t m l post :
+    exec c1 true t m l
+      (postcond (fun q' t' m' l' =>
+                   exec c2 q' t' m' l' post)) ->
+    exec (cmd.seq c1 c2) true t m l post.
+  Proof. intros. eapply seq_cps_sorta. 1: apply H. simpl. auto. Qed.
+
+  Lemma while_true_cps_sorta ee c t m l v prefix post :
+      eval_expr m l ee = Some v ->
+      word.unsigned v <> 0 ->
+      exec c true t m l prefix ->
+      sat prefix (exec (cmd.while ee c)) post ->
+      exec (cmd.while ee c) true t m l post.
+  Proof. intros. eapply while_true with (mid := exec _); eauto. Qed.
+
+  Open Scope string_scope.
+  Require Import Strings.String.
+  Definition ex := cmd.seq (cmd.set "x"%string (expr.literal 0)) (cmd.seq (cmd.set "x" (expr.literal 1)) (cmd.seq (cmd.set "x" (expr.literal 2)) cmd.skip)).
+
+  Context {locals_ok: map.ok locals} {word_ok: word.ok word} {mem_ok: map.ok mem} {ext_spec_ok: ext_spec.ok ext_spec}.
+
+  Lemma ex_works t m l : exec ex true t m l (and_then (fun _ _ _ l => map.get l "x" = Some (word.of_Z 0)) (fun _ _ _ _ _ => and_then (fun _ _ _ l => map.get l "x" = (Some (word.of_Z 1))) (fun _ _ _ _ _ => and_then (fun _ _ _ l => map.get l "x" = (Some (word.of_Z 2))) (fun _ _ _ _ _ => postcond (fun q _ _ _ => q = true))))).
+  Proof.
+    eapply seq_cps_sorta.
+    { eapply set. 1: reflexivity. instantiate (1 := fun q' t' m' l' => q' = true /\ map.get l' "x" = Some (word.of_Z 0)). simpl. rewrite map.get_put_same. auto. }
+    simpl. intros. fwd. eapply mid.
+    { assumption. }
+    intros _. eapply seq_cps_sorta.
+    { eapply set. 1: reflexivity. instantiate (1 := fun q' t' m' l' => q' = true /\ map.get l' "x" = Some (word.of_Z 1)). simpl. rewrite map.get_put_same. auto. }
+    simpl. intros. fwd. eapply mid.
+    { assumption. }
+    intros _. eapply seq_cps_sorta.
+    { eapply set. 1: reflexivity. instantiate (1 := fun q' t' m' l' => q' = true /\ map.get l' "x" = Some (word.of_Z 2)). simpl. rewrite map.get_put_same. auto. }
+    simpl. intros. fwd. eapply mid.
+    { assumption. }
+    intros _. apply skip. reflexivity.
+  Qed.
+  
   Lemma interact_cps: forall binds action arges args t m l post mKeep mGive,
       map.split m mKeep mGive ->
       eval_call_args m l arges = Some args ->
       ext_spec t mGive action args (fun mReceive resvals =>
           exists l', map.putmany_of_list_zip binds resvals l = Some l' /\
           forall m', map.split m' mKeep mReceive ->
-          post (cons ((mGive, action, args), (mReceive, resvals)) t) m' l') ->
-      exec (cmd.interact binds action arges) t m l post.
+          post true (cons ((mGive, action, args), (mReceive, resvals)) t) m' l') ->
+      exec (cmd.interact binds action arges) true t m l (postcond post).
   Proof. intros. eauto using interact. Qed.
+  
+  (* Lemma seq_cps: forall c1 c2 t m l post, *)
+  (*     exec c1 true t m l (fun q' t' m' l' => exec c2 q' t' m' l' post) -> *)
+  (*     exec (cmd.seq c1 c2) true t m l post. *)
+  (* Proof. intros. eauto using seq. Qed. *)
 
-  Lemma seq_cps: forall c1 c2 t m l post,
-      exec c1 t m l (fun t' m' l' => exec c2 t' m' l' post) ->
-      exec (cmd.seq c1 c2) t m l post.
-  Proof. intros. eauto using seq. Qed.
+  (*could be cleverer about this... seems unnecessary though*)
+  Fixpoint implies (post1 post2 : mids_and_post) :=
+    match post1, post2 with
+    | and_then mid1 post1', and_then mid2 post2' =>
+        (forall q' t' m' l', mid1 q' t' m' l' -> mid2 q' t' m' l') /\
+          (forall q' t' m' l' n, implies (post1' q' t' m' l' n) (post2' q' t' m' l' n))
+    | postcond post1', postcond post2' => forall q' t' m' l', post1' q' t' m' l' -> post2' q' t' m' l'
+    | _, _ => False
+    end.
 
-  Lemma weaken: forall t l m s post1,
-      exec s t m l post1 ->
-      forall post2,
-        (forall t' m' l', post1 t' m' l' -> post2 t' m' l') ->
-        exec s t m l post2.
+  Lemma weaken_sat post1 suffix_good1 suffix_good2 mid :
+    (forall q t m l post1 post2, implies post1 post2 -> suffix_good1 q t m l post1 -> suffix_good2 q t m l post2) ->
+    sat mid suffix_good1 post1 ->
+    forall post2,
+    implies post1 post2 ->
+    sat mid suffix_good2 post2.
   Proof.
-    induction 1; intros; try solve [econstructor; eauto].
+    intros. revert post1 post2 H0 H1. induction mid; intros.
+    - destruct post1; simpl in H0; destruct post2; simpl in H1; try solve [destruct H1].
+      + simpl. intros. apply H with (post1 := postcond post0); auto.
+      + simpl. intros. fwd. eapply H. 2: auto. simpl. auto.
+    - destruct post1; simpl in H1; try solve [destruct H1].
+      destruct post2; simpl in H2; try solve [destruct H2].
+      simpl. fwd. eauto.
+  Qed.
+
+  Lemma weaken: forall q t l m s post1,
+      exec s q t m l post1 ->
+      forall post2,
+        implies post1 post2 ->
+        exec s q t m l post2.
+  Proof.
+    induction 1; intros; simpl in *; fwd; try solve [econstructor; eauto].
+    - eapply seq_cps_sorta; eauto. eapply weaken_sat; eauto.
+    - eapply while_true_cps_sorta; eauto. eapply weaken_sat; eauto.
     - eapply stackalloc. 1: assumption.
-      intros.
-      eapply H1; eauto.
-      intros. fwd. eauto 10.
-    - eapply call.
-      4: eapply IHexec.
-      all: eauto.
-      intros.
-      edestruct H3 as (? & ? & ? & ? & ?); [eassumption|].
-      eauto 10.
+      intros. specialize (H0 _ _ _ ltac:(eassumption) ltac:(eassumption)).
+      fwd. exists prefix. split; [assumption|]. eapply weaken_sat; eauto.
+      simpl. intros. fwd. destruct post0; try solve [destruct H0].
+      exists post0. split; [reflexivity|]. simpl in H0. eauto 10.
+    (* - eapply call. *)
+    (*   4: eapply IHexec. *)
+    (*   all: eauto. *)
+    (*   intros. *)
+    (*   edestruct H3 as (? & ? & ? & ? & ?); [eassumption|]. *)
+    (*   eauto 10. *)
     - eapply interact; try eassumption.
       intros.
       edestruct H2 as (? & ? & ?); [eassumption|].
       eauto 10.
   Qed.
 
-  Lemma intersect: forall t l m s post1,
-      exec s t m l post1 ->
-      forall post2,
-        exec s t m l post2 ->
-        exec s t m l (fun t' m' l' => post1 t' m' l' /\ post2 t' m' l').
-  Proof.
-    induction 1;
-      intros;
-      match goal with
-      | H: exec _ _ _ _ _ |- _ => inversion H; subst; clear H
-      end;
-      try match goal with
-      | H1: ?e = Some (?x1, ?y1, ?z1), H2: ?e = Some (?x2, ?y2, ?z2) |- _ =>
-        replace x2 with x1 in * by congruence;
-          replace y2 with y1 in * by congruence;
-          replace z2 with z1 in * by congruence;
-          clear x2 y2 z2 H2
-      end;
-      repeat match goal with
-             | H1: ?e = Some ?v1, H2: ?e = Some ?v2 |- _ =>
-               replace v2 with v1 in * by congruence; clear H2
-             end;
-      repeat match goal with
-             | H1: ?e = Some ?v1, H2: ?e = Some ?v2 |- _ =>
-               replace v2 with v1 in * by congruence; clear H2
-             end;
-      try solve [econstructor; eauto | exfalso; congruence].
-
-    - econstructor. 1: eassumption.
-      intros.
-      rename H0 into Ex1, H11 into Ex2.
-      eapply weaken. 1: eapply H1. 1,2: eassumption.
-      1: eapply Ex2. 1,2: eassumption.
-      cbv beta.
-      intros. fwd.
-      lazymatch goal with
-      | A: map.split _ _ _, B: map.split _ _ _ |- _ =>
-        specialize @map.split_diff with (4 := A) (5 := B) as P
-      end.
-      edestruct P; try typeclasses eauto. 2: subst; eauto 10.
-      eapply anybytes_unique_domain; eassumption.
-    - econstructor.
-      + eapply IHexec. exact H5. (* not H *)
-      + simpl. intros *. intros [? ?]. eauto.
-    - eapply while_true. 1, 2: eassumption.
-      + eapply IHexec. exact H9. (* not H1 *)
-      + simpl. intros *. intros [? ?]. eauto.
-    - eapply call. 1, 2, 3: eassumption.
-      + eapply IHexec. exact H15. (* not H2 *)
-      + simpl. intros *. intros [? ?].
-        edestruct H3 as (? & ? & ? & ? & ?); [eassumption|].
-        edestruct H16 as (? & ? & ? & ? & ?); [eassumption|].
-        repeat match goal with
-               | H1: ?e = Some ?v1, H2: ?e = Some ?v2 |- _ =>
-                 replace v2 with v1 in * by congruence; clear H2
-               end.
-        eauto 10.
-    - pose proof ext_spec.mGive_unique as P.
-      specialize P with (1 := H) (2 := H7) (3 := H1) (4 := H13).
-      subst mGive0.
-      destruct (map.split_diff (map.same_domain_refl mGive) H H7) as (? & _).
-      subst mKeep0.
-      eapply interact. 1,2: eassumption.
-      + eapply ext_spec.intersect; [ exact H1 | exact H13 ].
-      + simpl. intros *. intros [? ?].
-        edestruct H2 as (? & ? & ?); [eassumption|].
-        edestruct H14 as (? & ? & ?); [eassumption|].
-        repeat match goal with
-               | H1: ?e = Some ?v1, H2: ?e = Some ?v2 |- _ =>
-                 replace v2 with v1 in * by congruence; clear H2
-               end.
-        eauto 10.
-  Qed.
+  (* Lemma intersect: forall s q t m l post1, *)
+  (*     (forall t m l, post1 false t m l -> False) -> *)
+  (*     exec s q t m l post1 -> *)
+  (*     forall post2, *)
+  (*       (forall t m l, post2 false t m l -> False) -> *)
+  (*       exec s q t m l post2 -> *)
+  (*       exec s q t m l (fun q' t' m' l' => post1 q' t' m' l' /\ post2 q' t' m' l'). *)
+  (* Proof. *)
+  (*   intros * Hpost1. *)
+  (*   induction 1; *)
+  (*     intros post2 Hpost2 ?; *)
+  (*     match goal with *)
+  (*     | H: exec _ _ _ _ _ _ |- _ => inversion H; *)
+  (*                                 try solve [exfalso; eauto]; *)
+  (*                                 subst; clear H *)
+  (*     end; *)
+  (*     try match goal with *)
+  (*     | H1: ?e = Some (?x1, ?y1, ?z1), H2: ?e = Some (?x2, ?y2, ?z2) |- _ => *)
+  (*       replace x2 with x1 in * by congruence; *)
+  (*         replace y2 with y1 in * by congruence; *)
+  (*         replace z2 with z1 in * by congruence; *)
+  (*         clear x2 y2 z2 H2 *)
+  (*     end; *)
+  (*     repeat match goal with *)
+  (*            | H1: ?e = Some ?v1, H2: ?e = Some ?v2 |- _ => *)
+  (*              replace v2 with v1 in * by congruence; clear H2 *)
+  (*            end; *)
+  (*     repeat match goal with *)
+  (*            | H1: ?e = Some ?v1, H2: ?e = Some ?v2 |- _ => *)
+  (*              replace v2 with v1 in * by congruence; clear H2 *)
+  (*            end; *)
+  (*     try solve [econstructor; eauto | exfalso; congruence]. *)
+  (*   - econstructor. 1: eassumption. *)
+  (* Abort. (*this should be true, but looks like a few minutes of effort*) *)
+    (*   intros. *)
+    (*   rename H0 into Ex1, H12 into Ex2. *)
+    (*   eapply weaken. 1: eapply H1. 1,2: eassumption. *)
+    (*   { intros. fwd. eauto. } *)
+    (*   2: eapply Ex2. *)
+    (*   { simpl. intros. fwd. eauto. } *)
+    (*   1,2: eassumption. *)
+    (*   cbv beta. *)
+    (*   intros. fwd. *)
+    (*   lazymatch goal with *)
+    (*   | A: map.split _ _ _, B: map.split _ _ _ |- _ => *)
+    (*     specialize @map.split_diff with (4 := A) (5 := B) as P *)
+    (*   end. *)
+    (*   edestruct P; try typeclasses eauto. 2: subst; eauto 10. *)
+    (*   eapply anybytes_unique_domain; eassumption. *)
+    (* - econstructor. *)
+    (*   + eapply weaken. 1: eapply IHexec. *)
+  (*       --  *)
+  (*       exact H5. (* not H *) *)
+  (*     + simpl. intros *. intros [? ?]. eauto. *)
+  (*   - eapply while_true. 1, 2: eassumption. *)
+  (*     + eapply IHexec. exact H9. (* not H1 *) *)
+  (*     + simpl. intros *. intros [? ?]. eauto. *)
+  (*   - eapply call. 1, 2, 3: eassumption. *)
+  (*     + eapply IHexec. exact H16. (* not H2 *) *)
+  (*     + simpl. intros *. intros [? ?]. *)
+  (*       edestruct H3 as (? & ? & ? & ? & ?); [eassumption|]. *)
+  (*       edestruct H17 as (? & ? & ? & ? & ?); [eassumption|]. *)
+  (*       repeat match goal with *)
+  (*              | H1: ?e = Some ?v1, H2: ?e = Some ?v2 |- _ => *)
+  (*                replace v2 with v1 in * by congruence; clear H2 *)
+  (*              end. *)
+  (*       eauto 10. *)
+  (*   - pose proof ext_spec.mGive_unique as P. *)
+  (*     specialize P with (1 := H) (2 := H7) (3 := H1) (4 := H14). *)
+  (*     subst mGive0. *)
+  (*     destruct (map.split_diff (map.same_domain_refl mGive) H H7) as (? & _). *)
+  (*     subst mKeep0. *)
+  (*     eapply interact. 1,2: eassumption. *)
+  (*     + eapply ext_spec.intersect; [ exact H1 | exact H14 ]. *)
+  (*     + simpl. intros *. intros [? ?]. *)
+  (*       edestruct H2 as (? & ? & ?); [eassumption|]. *)
+  (*       edestruct H15 as (? & ? & ?); [eassumption|]. *)
+  (*       repeat match goal with *)
+  (*              | H1: ?e = Some ?v1, H2: ?e = Some ?v2 |- _ => *)
+  (*                replace v2 with v1 in * by congruence; clear H2 *)
+  (*              end. *)
+  (*       eauto 10. *)
+  (* Qed. *)
 
   End WithEnv.
-
-  Lemma extend_env: forall e1 e2,
-      map.extends e2 e1 ->
-      forall c t m l post,
-      exec e1 c t m l post ->
-      exec e2 c t m l post.
-  Proof. induction 2; try solve [econstructor; eauto]. Qed.
-
   End WithParams.
 End exec. Notation exec := exec.exec.
+
+Require Import coqutil.Word.SimplWordExpr.
+From Coq Require Import ZArith.
+From Coq Require Import Lia.
 
 Section WithParams.
   Context {width: Z} {BW: Bitwidth width} {word: word.word width} {mem: map.map word byte}.
   Context {locals: map.map String.string word}.
-  Context {ext_spec: ExtSpec}.
+  Context {word_ok : word.ok word} {mem_ok: map.ok mem}.
 
-  Implicit Types (l: locals) (m: mem) (post: trace -> mem -> list word -> Prop).
+  Instance ext_spec : ExtSpec := fun t m action args post =>
+                                   post map.empty nil.
 
-  Definition call e fname t m args post :=
-    exists argnames retnames body,
-      map.get e fname = Some (argnames, retnames, body) /\
-      exists l, map.of_list_zip argnames args = Some l /\
-        exec e body t m l (fun t' m' l' => exists rets,
-          map.getmany_of_list l' retnames = Some rets /\ post t' m' rets).
+  Definition example := cmd.while (expr.literal 1) (cmd.interact nil String.EmptyString nil).
 
-  Lemma weaken_call: forall e fname t m args post1,
-      call e fname t m args post1 ->
-      forall post2, (forall t' m' rets, post1 t' m' rets -> post2 t' m' rets) ->
-      call e fname t m args post2.
+  Lemma one_not_zero : word.unsigned (word := word) (word.of_Z 1) <> 0.
   Proof.
-    unfold call. intros. fwd.
-    do 4 eexists. 1: eassumption.
-    do 2 eexists. 1: eassumption.
-    eapply exec.weaken. 1: eassumption.
-    cbv beta. clear -H0. intros. fwd. eauto.
+    rewrite word.unsigned_of_Z. cbv [word.wrap]. 
+    destruct word_ok. clear - width_pos.
+    assert (2 ^ 1 <= 2 ^ width).
+    { Search (_ ^ _ <= _ ^ _).  apply Z.pow_le_mono_r; lia. }
+    replace (2 ^ 1) with 2 in H by reflexivity.
+    remember (2 ^ width) as blah. clear Heqblah.
+    Fail Z.div_mod_to_equations; lia. (*?*)
+    rewrite Z.mod_small by lia. lia.
+  Qed.
+  
+  Require Import Strings.String.
+  Open Scope string_scope.
+  Definition one : LogItem := ((map.empty, "1", nil), (map.empty, nil)).
+  Import exec.
+  Definition eventually_always_one :=
+    exec.and_then (fun q' t' m' l' => True)
+      (fun q' t' m' l' =>
+       fun n =>
+         exec.postcond (fun q'' t'' m'' l'' =>
+                     t'' = (repeat one n ++ t')%list)).
+  
+  Definition eventually_always_one' (f : nat -> state) :=
+    exists m, forall n,
+    exists numsteps,
+      (f numsteps).(t) = (repeat one n ++ (f m).(t))%list.
+
+  Lemma eventually_always_one_right : forall f,
+      interp_mids_and_post eventually_always_one f <-> eventually_always_one' f.
+  Proof.
+    intros. cbv [eventually_always_one eventually_always_one']. simpl. split; intros; fwd.
+    - exists n. intros n0. specialize (Hp1 n0). fwd. exists n1.
+      cbv [state_satisfies appl_to_state] in Hp1. assumption.
+    - exists m0. split; [reflexivity|]. intros m. specialize (H m).
+      fwd. exists numsteps. cbv [state_satisfies appl_to_state]. assumption.
   Qed.
 
-  Lemma extend_env_call: forall e1 e2,
-      map.extends e2 e1 ->
-      forall f t m rets post,
-      call e1 f t m rets post ->
-      call e2 f t m rets post.
+  (*stackalloc 0 as x;
+    while x-- { print 1 }
+    while true { print 0 }*) Print expr.
+  Definition countdown :=
+    (cmd.while (expr.var "x")
+                  (cmd.seq
+                     (cmd.interact nil "0" nil)
+                     (cmd.set "x" (expr.op bopname.sub (expr.var "x") (expr.literal 1))))).
+
+  Context {locals_ok: map.ok locals}.
+
+  Lemma countdown_terminates t m l xval :
+    map.get l "x" = Some (word.of_Z xval) ->
+    0 <= xval ->
+    exec countdown true t m l (postcond (fun q' _ _ _ => q' = true)).
   Proof.
-    unfold call. intros. fwd. repeat eexists.
-    - eapply H. eassumption.
-    - eassumption.
-    - eapply exec.extend_env; eassumption.
+    intros. replace xval with (Z.of_nat (Z.to_nat xval)) in * by lia. clear H0.
+    remember (Z.to_nat xval) as xval'.
+    clear Heqxval' xval.
+    remember xval' as upper_bound.
+    rewrite Hequpper_bound in H.
+    assert (xval' <= upper_bound)%nat  by lia. clear Hequpper_bound. revert xval' H0 H.
+    revert t m l.
+    induction upper_bound; intros.
+    - eapply while_false.
+      + simpl. rewrite H. reflexivity.
+      + rewrite word.unsigned_of_Z. replace xval' with 0%nat by lia. reflexivity.
+      + reflexivity.
+    - assert (word.wrap (Z.of_nat xval') <> 0 \/ word.wrap (Z.of_nat xval') = 0) by lia.
+      destruct H1.
+      + eapply while_true_cps_sorta.
+        -- simpl. apply H.
+        -- rewrite word.unsigned_of_Z. assumption.
+        -- eapply seq_cps_sorta.
+           ++ eapply interact_cps.
+              --- apply map.split_empty_r. reflexivity.
+              --- reflexivity. 
+              --- cbv [ext_spec]. eexists. intuition eauto.
+                  instantiate (1 := fun q' _ _ l' => q' = true /\ map.get l' "x" = Some (word.of_Z (Z.of_nat xval'))). simpl. auto.
+           ++ simpl. intros. fwd. eapply set.
+              --- simpl. rewrite H2p1. reflexivity.
+              --- instantiate (1 := fun q' _ _ l' => q' = true /\ map.get l' "x" = Some _). simpl. intuition auto. rewrite map.get_put_same. reflexivity.
+        -- simpl. intros. fwd. eapply IHupper_bound.
+           2: { rewrite H2p1. f_equal.
+                instantiate (1 := Z.to_nat (word.unsigned _)). rewrite Z2Nat.id.
+                2: { epose proof Properties.word.unsigned_range _ as H2. apply H2. }
+                rewrite word.of_Z_unsigned. reflexivity. }
+           enough (word.unsigned (word := word) (word.sub (word.of_Z (Z.of_nat xval')) (word.of_Z 1)) <= Z.of_nat upper_bound) by lia.
+           pose proof Properties.word.decrement_nonzero_lt as H2.
+           specialize (H2 (word.of_Z (Z.of_nat xval'))).
+           rewrite word.unsigned_of_Z in H2. specialize (H2 H1).
+           remember (word.unsigned _) as blah. clear Heqblah. enough (word.wrap (Z.of_nat xval') <= 1 + (Z.of_nat upper_bound)) by lia.
+           clear H2 blah. cbv [word.wrap].
+           pose proof Z.mod_le (Z.of_nat xval') (2 ^ width) as H2.
+           specialize (H2 ltac:(lia)). eassert _ as blah. 2: specialize (H2 blah); lia.
+           assert (2 ^ 0 <= 2 ^ width).
+           { apply Z.pow_le_mono_r; try lia. destruct word_ok; clear - width_pos.
+             lia. }
+           lia.
+      + eapply while_false; eauto. rewrite word.unsigned_of_Z. assumption.
+  Qed.
+
+  Definition one_printer :=
+    (cmd.while (expr.literal 1) (cmd.interact nil "1" nil)).
+
+  Lemma one_printer_prints_ones n t m l :
+    exec one_printer true t m l
+      (postcond (fun q' t' m' l' => q' = false /\ t' = repeat one n ++ t)%nat%list).
+  Proof.
+    revert t m l. induction n; intros t m l.
+    - apply quit. simpl. auto.
+    - eapply while_true_cps_sorta.
+      + reflexivity.
+      + apply one_not_zero.
+      + eapply exec.interact_cps.
+        -- apply map.split_empty_r. reflexivity.
+        -- reflexivity.
+        -- cbv [ext_spec]. eexists. intuition eauto.
+           instantiate (1 := fun q' t' _ _ => q' = true /\ t' = one :: t).
+           simpl. auto.
+      + simpl. intros. fwd. eapply weaken. 1: apply IHn. simpl. intros.
+        fwd. intuition auto.
+        replace (repeat one n ++ one :: t)%list with (repeat one (S n) ++ t)%list.
+        -- reflexivity.
+        -- replace (S n) with (n + 1)%nat by lia. rewrite repeat_app.
+           rewrite <- app_assoc. reflexivity.
+  Qed.
+          
+  (* Lemma goes_forever e m l : *)
+  (*   forall n, *)
+  (*     exec e example true nil m l *)
+  (*       (fun q' t' m' l' => q' = false /\ length t' = n). *)
+  (* Proof. *)
+  (*   intros. eapply exec.weaken. 1: apply goes_forever'. simpl. intros. fwd. eauto. *)
+  (* Qed. *)
+
+  Definition eventual_one_printer :=
+    cmd.seq (cmd.stackalloc "x" 0 cmd.skip)
+      (cmd.seq countdown one_printer).
+
+  Lemma eventual_one_printer_eventually_always_one t m l : exec eventual_one_printer true t m l eventually_always_one.
+  Proof.
+    eapply seq_cps_sorta.
+    { eapply stackalloc. 1: apply Zmod_0_l; lia. intros. eexists. split.
+      { apply skip. instantiate (1 := fun q' t' m' l' => q' = true /\ t' = t /\ m' = mCombined /\ l' = map.put l "x" a). simpl. auto. }
+      simpl. intros. fwd. eexists. split; [reflexivity|].
+      eexists. eexists. split; [eassumption|]. split; [eassumption|].
+      instantiate (1 := fun q' t' m' l' => exists a, q' = true /\ t' = t /\ m' = m /\ l' = map.put l "x" a).
+      simpl. eauto. }
+    simpl. intros. fwd. eapply seq_cps_sorta.
+    { eapply countdown_terminates.
+      - rewrite map.get_put_same. instantiate (1 := word.unsigned _). rewrite word.of_Z_unsigned. reflexivity.
+      - pose proof Properties.word.unsigned_range a. lia. }
+    simpl. intros. subst.
+    (*Note: below gets stuck, as i guess it should*)
+    (*eapply weaken. 1: apply one_printer_prints_ones. simpl.*)
+    apply mid. 1: auto. intros n. eapply weaken.
+    - apply (one_printer_prints_ones n).
+    - simpl. intros. fwd. reflexivity.
+  Qed.
+
+  Lemma nested_quit t m l : exec (cmd.seq cmd.skip cmd.skip) true t m l (postcond (fun _ _ _ _ => True)).
+  Proof.
+    eapply seq_cps_for_real.
+    apply exec.quit.
+    Fail apply exec.skip. (*as it should be: cannot quit and then start executing again*)
+    apply exec.quit.
+    exact I.
   Qed.
 End WithParams.
